Add latex file and do second version of exercise

weakmem.v
@@ -102,3 +102,108 @@ Section mp_spec.
 End mp_spec.
 
 
+Section mp_code_alt.
+  (* Let's try another variation of the code: one where we read x and y only
+     _after_ both threads are done and, further, we read _both_ of their values. *)
+
+  Definition mp_alt : val :=
+    λ: <>,
+       let: "x" := ref #0 in
+       let: "y" := ref #0 in
+       let: "tmp" := (("x" <- #37;; "y" <- #1) ||| (repeat_prog "y";; #())) in
+       let: "res" := ref (!"x", !"y") in
+       "res".
+
+End mp_code_alt.
+
+Section mp_alt_model.
+
+  Definition stateRes (γ : gname) : iProp := own γ (Excl ()).
+
+  Variable l_out l_in : loc.
+  Variable γ1 γ2 γ3 : gname.
+  
+  Definition st1 : iProp :=
+    (l_out ↦ #0 ∗ l_in ↦ #0 ∗ stateRes γ2 ∗ stateRes γ3)%I.
+
+   Definition st2 : iProp :=
+     (l_out ↦ #0 ∗ l_in ↦ #37 ∗ stateRes γ1 ∗ stateRes γ3)%I.
+
+   Definition st3 : iProp :=
+    (l_out ↦ #1 ∗ l_in ↦ #37 ∗ stateRes γ1 ∗ stateRes γ2)%I. 
+  
+  Definition inv_alt : iProp := (st1 ∨ st2 ∨ st3)%I.
+
+End mp_alt_model.
+
+Section mp_alt_spec.
+
+  Definition mpName : namespace := nroot .@ "mp".
+
+    
+  Lemma mp_alt_spec :
+    {{{ True }}} mp_alt #() {{{ v, RET #v ; v ↦ (#37, #1) }}}.
+  Proof.
+    iIntros (ϕ) "_ Post".
+    rewrite /mp_alt. wp_pures.
+    wp_alloc lx as "Hx". wp_alloc ly as "Hy". wp_pures. wp_bind (par _ _).
+    iMod (own_alloc (Excl ())) as (γ1) "Hγ1"; try done.
+    iMod (own_alloc (Excl ())) as (γ2) "Hγ2"; try done.
+    iMod (own_alloc (Excl ())) as (γ3) "Hγ3"; try done.
+    iMod (inv_alloc mpName _ (inv_alt ly lx γ1 γ2 γ3) with "[Hγ2 Hγ3 Hx Hy]") as "#Hinv".
+    { iNext. iLeft. rewrite /st1.
+      rewrite /stateRes.
+      iFrame. }
+    wp_apply (wp_par (λ _, stateRes γ3)%I (λ vx, True)%I with "[Hγ1] []").
+    - wp_bind (_ <- _)%E.
+      iInv mpName as "> [(Hx & Hy & Hst2 & Hst3) | [(_ & _ & Hst1 & _) | (_ & _ & Hst1 & _)]]" "Hclose"; rewrite /stateRes.
+      2: { by iExFalso; iDestruct (own_valid_2 with "Hγ1 Hst1") as %Hv. }
+      2: { by iExFalso; iDestruct (own_valid_2 with "Hγ1 Hst1") as %Hv. }
+      wp_store. iMod ("Hclose" with "[Hx Hy Hγ1 Hst3]") as "_".
+      { iNext. rewrite /inv_alt. iRight. iLeft. iFrame. }
+      iModIntro. wp_pures.
+      iInv mpName as "> [(_ & _ & Hγ2 & _) | [(Hy & Hx & Hst1 & Hst3) | (_ & _ & _ & Hγ2)]]" "Hclose"; rewrite /stateRes.
+      { by iExFalso; iDestruct (own_valid_2 with "Hγ2 Hst2") as %Hv. }
+      2 : {  by iExFalso; iDestruct (own_valid_2 with "Hγ2 Hst2") as %Hv. }
+      wp_store. iMod ("Hclose" with "[Hx Hy Hst1 Hst2]") as "_".
+      { iNext. iRight. iRight. iFrame. }
+      iModIntro. iFrame.
+    - iLöb as "IH".
+      rewrite /repeat_prog. wp_pures. wp_bind (!_)%E.
+      iInv mpName as "> [(Hy & Hx & Hst2 & Hst3) | [(Hy & Hx & Hst1 & Hst3) | (Hy & Hx & Hst1 & Hst2)]]" "Hclose"; rewrite /stateRes.
+      + wp_load. iMod ("Hclose" with "[Hy Hx Hst2 Hst3]") as "_".
+        iNext. rewrite /inv_alt. iLeft. iFrame.
+        iModIntro.
+        wp_let. wp_pure _. wp_pure _.
+        iApply "IH".
+      + wp_load. iMod ("Hclose" with "[Hy Hx Hst1 Hst3]") as "_".
+        iNext. rewrite /inv_alt. iRight. iLeft. iFrame.
+        iModIntro.
+        wp_let. wp_pure _. wp_pure _.
+        iApply "IH".
+      + wp_load. iMod ("Hclose" with "[Hy Hx Hst1 Hst2]") as "_".
+        { iNext. rewrite /inv_alt. iRight. iRight. iFrame. }
+        iModIntro.
+        wp_pures. done.
+    - iIntros (v1 v2) "[Hst3 _]".
+      iNext. wp_pures. wp_bind (!#ly)%E.
+      iInv mpName as "> [(_ & _ & _ & Hγ3) | [(_ & _ & _ & Hγ3) | (Hy & Hx & Hst1 & Hst2)]]" "Hclose"; rewrite /stateRes.
+      {  by iExFalso; iDestruct (own_valid_2 with "Hγ3 Hst3") as "%". }
+      {  by iExFalso; iDestruct (own_valid_2 with "Hγ3 Hst3") as "%". }
+      wp_load. iMod ("Hclose" with "[Hy Hx Hst1 Hst2]") as "_".
+      { iNext. rewrite /inv_alt. iRight. iRight. iFrame. }
+      iModIntro.
+      wp_bind (!#lx)%E.
+      iInv mpName as "> [(_ & _ & _ & Hγ3) | [(_ & _ & _ & Hγ3) | (Hy & Hx & Hst1 & Hst2)]]" "Hclose"; rewrite /stateRes.
+      {  by iExFalso; iDestruct (own_valid_2 with "Hγ3 Hst3") as "%". }
+      {  by iExFalso; iDestruct (own_valid_2 with "Hγ3 Hst3") as "%". }
+      wp_load. iMod ("Hclose" with "[Hy Hx Hst1 Hst2]") as "_".
+      { iNext. rewrite /inv_alt. iRight. iRight. iFrame. }
+      iModIntro.
+      wp_pures. wp_alloc lp as "Hp".
+      wp_pures.
+      iApply "Post".
+      iFrame.
+  Qed.
+
+End mp_alt_spec.
